Migrated everything to the inductive representation

Metatheory.v
@@ -4,452 +4,105 @@ Require Import SysF.
 Require Import Arith.
 Require Import Omega.
 
-Lemma cumulativity : forall e : env, forall t : typ, forall k k' : kind,
-                       kinding e t k -> k <= k' -> kinding e t k'.
-  intro e0. intro t. generalize e0 as e. clear e0. (* This is ugly *)
-  induction t.
-  - intros.
-      simpl.
-      simpl in H.
-      remember (get_kind e n) as k1 in H |- *.
-      destruct k1.
-      + split. apply H. destruct H. omega.
-      + apply H.
-  - intros.
-    simpl in H.
-    do 3 destruct H. destruct H1.
-    simpl.
-    exists k'. exists k'.
-    split. auto with arith. split.
-    apply (IHt1 e x). trivial. assert (x <= max x x0). auto with arith. omega.
-    apply (IHt2 e x0). trivial. assert (x0 <= max x x0). auto with arith. omega.
-  - intros.
-    simpl.
-    do 2 destruct H.
-    exists (k' - k0 + (max x k)). split.
-    apply (IHt (etvar k e) x). apply H.
-    assert (x <= max x k). auto with arith. omega.
-    assert (max x k >= k). auto with arith. assert (k' - k0 + max x k >= k). omega.
-    assert (max (k' - k0 + max x k) k = (k' - k0+ max x k)). auto with arith. rewrite H4.
-    rewrite -> H1. assert (S (k' - S (max x k) + max x k) = k' - S (max x k) + S (max x k)).
-    rewrite (plus_comm (k' - S (max x k)) (S (max x k))). rewrite le_plus_minus_r. omega.
-    omega.
-    rewrite -> H5. rewrite (plus_comm). rewrite le_plus_minus_r. trivial.
-    rewrite <- H1. apply H0.
-Qed.
+Inductive insert_kind : nat -> env -> env -> Prop :=
+| ik_top kind env :
+    insert_kind 0 env (etvar kind env)
+| ik_evar pos typ env env' :
+    insert_kind pos env env' ->
+    insert_kind pos (evar typ env) (evar (tshift pos typ) env')
+| ik_etvar pos kind env env' :
+    insert_kind pos env env' ->
+    insert_kind (S pos) (etvar kind env) (etvar kind env')
+.
 
-Fixpoint insert_kind_r (i : nat) (v : nat) (e : env) (e' : env) : Prop :=
-  match e with
-    | evar t e1 =>
-      match e' with
-        | evar t' e1' => (tshift v t) = t' /\ insert_kind_r i v e1 e1'
-        | _ => False
-      end
-    | etvar k e1 =>
-      match e' with
-        | etvar k' e1' =>
-          match i with
-            | 0 => etvar k e1 = e1'
-            | S i1 => k = k' /\ insert_kind_r i1 v e1 e1'
-          end
-        | _ => False
-      end
-    | empty =>
-      match e' with
-        | etvar k empty => v = 0
-        | _ => False
-      end
-  end.
-
-Definition insert_kind (v : nat) := insert_kind_r v v.
-
-Hint Transparent insert_kind : core.
-Hint Transparent insert_kind_r : core.
-Hint Unfold insert_kind : core.
-Hint Unfold insert_kind_r : core.
-
-Definition shift_var (v : nat) (i : nat) :=
-  if le_gt_dec i v
-  then S v
-  else v.
-
-Lemma shift_var_s : forall (v i : nat), shift_var (S v) (S i) = S (shift_var v i).
-  induction v.
-  - destruct i; [ simpl; compute; trivial .. ].
-  - destruct i.
-    + compute. trivial.
-    + specialize (IHv i).
-      unfold shift_var in IHv |- *.
-      remember (le_gt_dec (S i) (S v)).
-      remember (le_gt_dec (S (S i)) (S (S v))).
-      destruct s.
-      * destruct s0.
-        { reflexivity. }
-        { exfalso. omega. }
-      * destruct s0.
-        { exfalso. omega. }
-        { reflexivity. }
-Qed.
-
-Lemma insert_kind_get_kind_lt : forall (e e' : env), forall (i v : nat),
-                                  insert_kind_r i v e e' ->
-                                  forall (w : nat),
-                                    w < i ->
-                                    match get_kind e w with
-                                      | Some k => get_kind e' w = Some k
-                                      | None => True
-                                    end.
-  induction e.
-  - intros. simpl. trivial.
-  - intros. simpl. destruct e'.
-    + inversion H.
-    + simpl. apply (IHe e' i v). simpl in H. apply H. apply H0.
-    + inversion H.
-  - intros. destruct e'. 
-    + inversion H.
-    + inversion H.
-    + destruct w.
-      * destruct i.
-        { omega. }
-        { destruct H. rewrite H. simpl. trivial. }
-      * destruct i.
-        { omega. }
-        { simpl. apply (IHe e' i v). apply H. omega. }
-Qed.
-
-Lemma insert_kind_get_kind_ge : forall (e e' : env), forall (i v : nat),
-                                  insert_kind_r i v e e' ->
-                                  forall (w : nat),
-                                    w >= i ->
-                                    match get_kind e w with
-                                      | Some k => get_kind e' (S w) = Some k
-                                      | None => True
-                                    end.
-  induction e.
-  - intros. simpl. trivial.
-  - intros. simpl. destruct e'.
-    + inversion H.
-    + simpl. apply (IHe e' i v). simpl in H. apply H. apply H0.
-    + inversion H.
-  - intros. destruct e'. 
-    + inversion H.
-    + inversion H.
-    + destruct w.
-      * destruct i.
-        { simpl in H. rewrite H. simpl. destruct (get_kind e' 0). simpl. trivial. trivial. }
-        { omega. }
-      * destruct i.
-        { simpl in H. rewrite H. simpl. destruct (get_kind e' (S w)). trivial. trivial. }
-        { simpl. apply (IHe e' i v). apply H. omega. }
-Qed.
-        
-Lemma insert_kind_get_kind : forall (e e' : env), forall (i v : nat),
-                               insert_kind_r i v e e' ->
-                               forall (w : nat),
-                                 match get_kind e w with
-                                   | Some k => get_kind e' (shift_var w i) = Some k
-                                   | None => True
-                                 end.
+Lemma shift_var_s : forall var shift,
+                      (if le_gt_dec (S shift) (S var) then S (S var) else S var) =
+                      S (if le_gt_dec shift var then S var else var).
   intros.
-  unfold shift_var.
-  destruct (le_gt_dec i w).
-  - apply (insert_kind_get_kind_ge e e' i v H w l).
-  - apply (insert_kind_get_kind_lt e e' i v H w g).
+  induction var.
+  - destruct shift; [ auto .. ].
+  - destruct (le_gt_dec shift var) eqn:shift_le_var,
+             (le_gt_dec (S shift) (S (S var))) eqn:Sshift_le_SSvar,
+             (le_gt_dec shift (S var)) eqn:shift_le_Svar;
+    [ omega .. ].
 Qed.
 
-Definition exists_kind (e : env) (n : nat) := match get_kind e n with Some _ => True | None => False end.
-Hint Transparent exists_kind : core.
-Hint Unfold exists_kind : core.
-
-Fixpoint highest_free_typ_variable (t : typ) :=
-  match t with
-    | tvar n => Some n
-    | tarr t1 t2 => match highest_free_typ_variable t1 with
-                      | None => highest_free_typ_variable t2
-                      | Some h1 => match highest_free_typ_variable t2 with
-                                     | None => Some h1
-                                     | Some h2 => if le_gt_dec h1 h2 then Some h2 else Some h1
-                                   end
-                    end
-    | tall _ t1 => match highest_free_typ_variable t1 with
-                     | None => None
-                     | Some 0 => None
-                     | Some (S n) => Some n
-                   end
-  end.
-
-Fixpoint num_typ_variables (e : env) :=
-  match e with
-    | empty => 0
-    | etvar _ e' => S (num_typ_variables e')
-    | evar _ e => num_typ_variables e
-  end.
-
-Lemma get_free_variable : forall e, forall n,
-                            n < num_typ_variables e <-> exists_kind e n.
-  induction e.
-  - simpl. intros. split. omega. intro. inversion H.
-  - intros. split.
-    + intro. simpl in H |- *. apply IHe. apply H.
-    + unfold exists_kind. simpl. apply IHe.
-  - intros. split.
-    + intro. unfold exists_kind.  simpl in H.
-      destruct n.
-      * simpl. trivial.
-      * apply IHe. auto with arith.
-    + intro. destruct n.
-      * simpl. auto with arith.
-      * simpl in H |- *. apply lt_n_S. apply IHe. apply H.
+Hint Rewrite shift_var_s : core.
+    
+Lemma insert_kind_get_kind : forall pos e e',
+                               insert_kind pos e e' ->
+                               forall var,
+                                 get_kind e var = get_kind e' (if le_gt_dec pos var then S var else var).
+  do 4 intro.
+  induction H.
+  - auto with arith.
+  - auto.
+  - destruct var.
+    + auto.
+    + rewrite shift_var_s. eauto.
 Qed.
 
-Lemma num_typ_variables_significant : forall (t : typ), forall (e : env),
-                                        wf_typ e t <->
-                                        match highest_free_typ_variable t with
-                                          | None => True
-                                          | Some i => i < num_typ_variables e
-                                        end.
-  split. generalize e. clear e. {
-  induction t.
-  - intros. simpl. apply get_free_variable. apply H.
-  - intros. simpl. destruct (highest_free_typ_variable t1); destruct (highest_free_typ_variable t2).
-    + destruct (le_gt_dec n n0).
-      * apply IHt2. apply H.
-      * apply IHt1. apply H.
-    + apply IHt1. apply H.
-    + apply IHt2. apply H.
-    + trivial.
-  - intros. simpl in H.
-    simpl. remember (highest_free_typ_variable t). destruct (highest_free_typ_variable t).
-    + rewrite Heqo in IHt |- *. destruct n.
-      * trivial.
-      * assert (S n < num_typ_variables (etvar k e) -> n < num_typ_variables e). simpl. auto with arith.
-        apply H0. apply (IHt (etvar k e) H).
-    + rewrite -> Heqo. trivial.
-  } 
-                                generalize e. clear e. induction t.
-  - intros. apply get_free_variable. apply H.
-  - intros. simpl in H. destruct (highest_free_typ_variable t1); destruct (highest_free_typ_variable t2).
-    + destruct (le_gt_dec n n0). 
-      * split. { apply IHt1. omega. } { apply IHt2. omega. }
-      * split. { apply IHt1. omega. } { apply IHt2. omega. } 
-    + split. { apply IHt1, H. } { apply IHt2. trivial. }
-    + split. { apply IHt1. trivial. } { apply IHt2, H. }
-    + split. { apply IHt1. trivial. } { apply IHt2. trivial. }
-  - intros. simpl. apply IHt. remember (highest_free_typ_variable (tall k t)) in H.
-    destruct o. simpl in Heqo.
-    destruct (highest_free_typ_variable t).
-    + destruct n0. inversion Heqo. simpl. apply lt_n_S. inversion Heqo. rewrite <- H1. apply H.
-    + trivial.
-    + simpl. simpl in Heqo. destruct (highest_free_typ_variable t). 
-      * destruct n. auto with arith. inversion Heqo.
-      * trivial.
-Qed.
-
-Lemma num_typ_variables_insert_kind : forall e e' i n,
-                                        insert_kind_r i n e e'
-                                        -> num_typ_variables e' = S (num_typ_variables e).
-  unfold insert_kind.
-  induction e.
-  - intros. destruct e'. inversion H. inversion H.
-    + destruct e'. trivial. inversion H. inversion H.
-  - intros. destruct e'. 
-    + inversion H.
-    + simpl in H. apply (IHe e' i n). apply H. 
-    + inversion H.
-  - intros. destruct e'. inversion H. inversion H.
-    destruct i.
-    + simpl in H. rewrite <- H. simpl. trivial.
-    + simpl. simpl in H. specialize (IHe e' i n).
-      assert (num_typ_variables e' = S (num_typ_variables e)). apply IHe. apply H. congruence.
-Qed.
-
-Lemma highest_free_typ_variable_tshift_s
-: forall t v, match highest_free_typ_variable (tshift (S v) t) with
-                | Some n1 =>
-                  match highest_free_typ_variable (tshift v t) with
-                    | None => n1 = 0
-                    | Some n2 => n1 <= S n2
-                  end
-                | None => True
-              end.
-  induction t.
-  - intros. unfold tshift. destruct (le_gt_dec v n); destruct (le_gt_dec (S v) n).
-    + simpl. auto with arith. + simpl. auto with arith. + simpl. trivial. + simpl. auto with arith.
-  - intros. specialize (IHt1 v). specialize (IHt2 v).
-    simpl. destruct (highest_free_typ_variable (tshift (S v) t1));
-      destruct (highest_free_typ_variable (tshift (S v) t2)).
-    + destruct (highest_free_typ_variable (tshift (v) t1));
-      destruct (highest_free_typ_variable (tshift (v) t2)).
-      destruct (le_gt_dec n n0); destruct (le_gt_dec n1 n2). 
-      omega. omega. omega. omega. destruct (le_gt_dec n n0). omega. omega.
-      destruct (le_gt_dec n n0). omega. omega. destruct (le_gt_dec n n0). omega. omega.
-    + destruct (highest_free_typ_variable (tshift v t1)).
-      destruct (highest_free_typ_variable (tshift v t2)).
-      destruct (le_gt_dec n0 n1). omega. omega. omega.
-      destruct (highest_free_typ_variable (tshift v t2)).
-      omega. omega.
-    + destruct (highest_free_typ_variable (tshift v t2)).
-      destruct (highest_free_typ_variable (tshift v t1)).
-      destruct (le_gt_dec n1 n0). omega. omega. omega.
-      destruct (highest_free_typ_variable (tshift v t1)).
-      omega. omega.
-    + trivial.
-  - intros. simpl. specialize (IHt (S v)).
-    destruct (highest_free_typ_variable (tshift (S v) t)).
-    + destruct (highest_free_typ_variable (tshift (S (S v)) t)).
-      * destruct n.
-        { destruct n0. trivial. omega. }
-        { destruct n0. trivial. omega. }
-      * trivial.
-    + destruct (highest_free_typ_variable (tshift (S (S v)) t)).
-      * destruct n. trivial. inversion IHt.
-      * trivial.
-Qed.
-
-Lemma highest_free_variable_tshift
-: forall t v, match highest_free_typ_variable t with
-                | None =>
-                  match highest_free_typ_variable (tshift v t) with
-                    | None => True
-                    | Some 0 => True
-                    | _ => False
-                  end
-                | Some t1 =>
-                    match highest_free_typ_variable (tshift v t) with
-                      | Some t2 => t2 <= S t1
-                      | None => True
-                    end
-              end.
-  induction t.
-  - intros. unfold tshift. destruct (le_gt_dec v n).
-    + simpl. trivial.
-    + simpl. auto with arith.
-  - intros. specialize (IHt1 v). specialize (IHt2 v).
-    simpl. destruct (highest_free_typ_variable t1); destruct (highest_free_typ_variable t2).
-    + destruct (le_gt_dec n n0).
-      * destruct (highest_free_typ_variable (tshift v t1));
-        destruct (highest_free_typ_variable (tshift v t2)).
-        destruct (le_gt_dec n1 n2).
-        { omega. } { omega. } { omega. } { omega. } { trivial. }
-      * destruct (highest_free_typ_variable (tshift v t1));
-        destruct (highest_free_typ_variable (tshift v t2)).
-        destruct (le_gt_dec n1 n2).
-        { omega. } { omega. } { omega. } { omega. } { trivial. }
-    + destruct (highest_free_typ_variable (tshift v t1));
-      destruct (highest_free_typ_variable (tshift v t2)).
-      destruct (le_gt_dec n0 n1). destruct n1. omega. omega. omega. omega.
-      destruct n0; [trivial | auto]. omega. omega. trivial.
-    + destruct (highest_free_typ_variable (tshift v t1));
-      destruct (highest_free_typ_variable (tshift v t2)).
-      destruct (le_gt_dec n0 n1). destruct n1. omega. omega.
-      destruct n0. omega. omega. destruct n0. omega. omega. omega. trivial.
-    + destruct (highest_free_typ_variable (tshift v t1));
-      destruct (highest_free_typ_variable (tshift v t2)).
-      destruct (le_gt_dec n n0). apply IHt2. apply IHt1. apply IHt1. apply IHt2. trivial.
-  - intros. simpl. pose proof (highest_free_typ_variable_tshift_s t v).
-    destruct (highest_free_typ_variable t). 
-    + specialize (IHt (S v)). destruct n.
-      * destruct (highest_free_typ_variable (tshift (S v) t)).
-        destruct n. trivial. destruct n. trivial. omega. trivial.
-      * destruct (highest_free_typ_variable (tshift (S v) t)).
-        destruct n0. trivial. destruct (highest_free_typ_variable (tshift v t)). omega. omega. trivial.
-    + specialize (IHt (S v)). destruct (highest_free_typ_variable (tshift (S v) t)). destruct n.
-      * trivial. * inversion IHt. * trivial.
-Qed.
-                                   
-Lemma insert_kind_wf_typ : forall (t : typ), forall (e e' : env), forall (i v : nat),
-                             insert_kind_r i v e e' ->
-                             wf_typ e t -> wf_typ e' (tshift v t).
-  intros.
-  pose proof (highest_free_variable_tshift t v).
-  pose proof (num_typ_variables_insert_kind e e' i v H).
-  pose proof (num_typ_variables_significant (tshift v t) e').
-  pose proof (num_typ_variables_significant t e).
-  rewrite H2 in H3. destruct H3. apply H5.
-  apply num_typ_variables_significant in H5.
-  - destruct (highest_free_typ_variable (tshift v t)).
-    + destruct (highest_free_typ_variable t).
-      * omega. * omega.
-    + trivial.
-  - destruct (highest_free_typ_variable (tshift v t)).
-    + destruct (highest_free_typ_variable t).
-      apply H4 in H0. omega. destruct n. omega. inversion H1.
-    + trivial.
-Qed.
-
-Theorem insert_kind_wf_env_r :
-  forall (i v : nat), forall (e e' : env), insert_kind_r i v e e' -> wf_env e -> wf_env e'.
-  intros until e. generalize i, v. clear i. clear v.
-  induction e.
-  - intros. destruct e'.
-    + inversion H.
-    + inversion H.
-    + simpl in H. destruct e'.
-      * trivial.
-      * inversion H.
-      * inversion H.
-  - intros. destruct e'.
-    + simpl. trivial.
-    + simpl. split. 
-      * simpl in H.
-        simpl in H0.
-        destruct H.
-        rewrite <- H.
-        apply (insert_kind_wf_typ t e e' i v H1).
-        apply H0.
-      * apply (IHe i v). apply H. apply H0.
-    + inversion H.
-  - intros. destruct e'.
-    + simpl. trivial.
-    + inversion H.
-    + destruct i.
-      * simpl in H. rewrite <- H. simpl. apply H0.
-      * simpl in H. simpl. apply (IHe i v e'). apply H. apply H0.
-Qed.
-
-Theorem insert_kind_wf_env : forall v, forall e e', insert_kind v e e' -> wf_env e -> wf_env e'.
-  intros.
-  apply (insert_kind_wf_env_r v v e e'); [auto..].
-Qed.
-
-Theorem insert_kind_kinding_r : forall (i v : nat), forall (e e' : env), forall (t : typ), forall (k : kind),
-                                  insert_kind_r i v e e' -> kinding e t k -> kinding e' (tshift i t) k.
-  intros until t. generalize i, v, e, e'. clear i. clear v. clear e. clear e'.
-  induction t.
+Theorem insert_kind_wf_typ : forall pos e e' typ,
+                               insert_kind pos e e' ->
+                               wf_typ e typ -> wf_typ e' (tshift pos typ).
+  intros until typ. generalize pos e e'. clear pos. clear e. clear e'.
+  induction typ.
   - intros.
-    simpl. simpl in H0.
-    assert ((if le_gt_dec i n then S n else n) = shift_var n i). auto.
-    rewrite -> H1.
-    pose proof (insert_kind_get_kind e e' i v H n). 
-    destruct (get_kind e n).
-    + rewrite -> H2.
-      split.
-      * apply (insert_kind_wf_env_r i v e e'). auto. apply H0.
-      * apply H0.
-    + inversion H0.
-  - intros. simpl.
-    do 2 destruct H0.
-    exists x. exists x0.
+    simpl. erewrite <- insert_kind_get_kind; [ eauto .. ].
+  - intros. destruct H0. split; [ eauto .. ].
+  - intros. simpl in H0. simpl.
+    eapply IHtyp.
+    eapply ik_etvar.
+    apply H.
+    apply H0.
+Qed.
+
+Theorem insert_kind_wf_env : forall pos e e',
+                               insert_kind pos e e' ->
+                               wf_env e -> wf_env e'.
+  do 4 intro.
+  induction H.
+  - auto.
+  - intro. simpl.
     split.
-    + apply H0.
-    + split.
-      * apply (IHt1 i v e). apply H. apply H0.
-      * apply (IHt2 i v e). apply H. apply H0.
-  - intros. simpl.
-    destruct H0.
-    exists x.
-    split.
-    + apply (IHt (S i) v (etvar k e)). simpl. split. trivial. apply H. apply H0.
-    + apply H0.
+    + eapply insert_kind_wf_typ.
+      apply H.
+      apply H0.
+    + apply IHinsert_kind.
+      apply H0.
+  - intro. apply IHinsert_kind. apply H0.
 Qed.
 
-Theorem insert_kind_get_typ_r : forall (e e' : env), forall (i v : nat), forall (n : nat),
-                                  insert_kind_r i v e e' ->
-                                  match get_typ e n with
-                                    | Some t => get_typ e' (shift_var i n) = Some (tshift v t)
-                                    | None => True
-                                  end.
-  induction e.
-  - intros. simpl. trivial.
-  - intros. destruct e'. inversion H.
-    + specialize (IHe e' i v n). destruct H.
+Theorem insert_kind_kinding : forall typ kind,
+                              forall pos e e',
+                                insert_kind pos e e' ->
+                                kinding e typ kind -> kinding e' (tshift pos typ) kind.
+  induction typ.
+  - intros. inversion H0.
+    eapply k_tvar.
+    { eapply insert_kind_wf_env; [ eauto .. ]. }
+    { erewrite <- insert_kind_get_kind; [ eauto .. ]. }
+    auto.
+  - intros. inversion H0.
+    eauto using k_tarr.
+  - intros. inversion H0.
+    eauto using ik_etvar, k_tall.
+Qed.
+
+Lemma insert_kind_get_typ : forall pos,
+                            forall var e e',
+                              insert_kind pos e e' ->
+                              wf_env e ->
+                              match get_typ e var with
+                                | None => get_typ e' var = None
+                                | Some t => get_typ e' var = Some (tshift pos t)
+                              end.
+  - intros until pos. generalize var. 
+    
+Theorem insert_kind_typing : forall term typ,
+                             forall pos e e',
+                               insert_kind pos e e' ->
+                               typing e term typ -> typing e' term (tshift pos typ).
+  induction term.
+  - intros. eapply t_var. inversion H0.
+    eapply insert_kind_wf_env. eauto. auto.
